theories/interop/weakestpre.v
@@ -51,7 +51,8 @@ Definition preGCtok : iProp Σ :=
   ∗ "GCζvirt" ∷ lstore_own_auth (∅:lstore)
   ∗ "GCML" ∷ state_interp (∅ : language.language.state ML_lang)
   ∗ "GCχvirt" ∷ lloc_own_auth (∅:lloc_map)
-  ∗ "GCrootsm" ∷ ghost_map_auth wrapperG_γroots_map 1 (∅:gmap addr lval).
+  ∗ "GCrootsm" ∷ ghost_map_auth wrapperG_γroots_global_map 1 (∅:gmap addr lval).
+  (* TODO: frame here ?*)
 
 Definition C_state_interp (ζ : lstore) (χ : lloc_map) (θ : addr_map) (roots_s : list $ gset addr) : iProp Σ :=
   ∃ (at_init : bool),
@@ -64,16 +65,20 @@ Definition C_state_interp (ζ : lstore) (χ : lloc_map) (θ : addr_map) (roots_s
   ∗ "Hinit" ∷ if at_init then preGCtok else True.
 
 Definition GC_remnant (ζ : lstore) (χ : lloc_map) (roots_m : list roots_map) : iProp Σ :=
-  ∃ (roots_f : list gname),
+  ∃ (roots_fm : list roots_map) (roots_gm : roots_map)
+    (roots_f : list gname),
    "GCζ" ∷ ghost_var wrapperG_γζ (1/2) ζ
  ∗ "GCχ" ∷ ghost_var wrapperG_γχ (1/2) χ
  ∗ "GCθ" ∷ ghost_var wrapperG_γθ (1/2) (∅:addr_map)
  ∗ "GCHGH" ∷ HGH χ None ζ
  ∗ "GCinit" ∷ ghost_var wrapperG_γat_init (1/2) false
  ∗ "GCroots" ∷ ghost_var wrapperG_γroots_set (1/2) (map dom roots_m)
- ∗ "GCrootsf"  ∷ghost_var wrapperG_γroots_frame (1 / 2) roots_f
- ∗ "GCrootsm" ∷ ([∗ list] f; r ∈ roots_f;roots_m, ghost_map_auth f 1 r)
- ∗ "GCrootspto" ∷ ([∗ list] r ∈ roots_m, [∗ set] a ∈ (dom r), a O↦C None).
+ ∗ "GCrootsf" ∷ ghost_var wrapperG_γroots_frame (1/2) roots_f
+ ∗ "GCrootsg" ∷ ghost_map_auth wrapperG_γroots_global_map 1 roots_gm
+ ∗ "GCrootsm" ∷ ([∗ list] f; r ∈ roots_f; roots_fm,
+                 ghost_map_auth f (1/2) r)
+ ∗ "GCrootspto" ∷ ([∗ list] r ∈ roots_m, [∗ set] a ∈ (dom r), a O↦C None)
+ ∗ "%GCrootsm" ∷ ⌜roots_m = roots_gm :: roots_fm⌝.
 
 Definition ML_state_interp (ζ : lstore) (χ : lloc_map) (roots_m : list roots_map) (memC : memory) : iProp Σ :=
     "SIζ" ∷ ghost_var wrapperG_γζ (1/2) ζ
