theories/interop/wp_prims/initlocalroot.v
@@ -4,7 +4,7 @@ From melocoton Require Import named_props stdpp_extra.
 From melocoton.mlanguage Require Import mlanguage.
 From melocoton.c_interface Require Import defs notation resources.
 From melocoton.interop Require Import state lang basics_resources.
-From melocoton.interop Require Export prims weakestpre prims_proto update_laws.
+From melocoton.interop Require Export prims weakestpre prims_proto wp_utils.
 From melocoton.interop.wp_prims Require Import common.
 From melocoton.mlanguage Require Import weakestpre.
 Import Wrap.
@@ -20,7 +20,7 @@ Context `{!wrapperG Σ}.
 Implicit Types P : iProp Σ.
 Import mlanguage.
 
-Lemma read_foreign_correct e : |- wrap_prog e :: read_foreign_proto.
+Lemma initlocalroot_correct e : |- wrap_prog e :: initlocalroot_proto.
 Proof using.
   iIntros (? ? ? ?) "H". unfold mprogwp. iNamedProto "H".
   iSplit; first done.
@@ -28,22 +28,8 @@ Proof using.
   rewrite weakestpre.wp_unfold. rewrite /weakestpre.wp_pre.
   iIntros "%σ Hσ". cbn -[wrap_prog].
   SI_at_boundary. iNamed "HGC". SI_GC_agree.
-  iAssert ⌜∃ m', ζC ρc !! γ = Some (Bforeign (m', Some w'))⌝%I as "%Helem2".
-  {
-    iDestruct "Hpto" as "[Hpto _]".
-    iDestruct (hgh_lookup_foreign with "GCHGH Hpto") as %(?&_&?). iPureIntro. eauto.
-  }
-  destruct Helem2 as [m' Helem2].
+
   iApply wp_pre_cases_c_prim; [done..|].
-  iExists (λ '(e', σ'), e' = WrSE (ExprO (OVal w')) ∧ σ' = CState ρc mem).
-  iSplit. { iPureIntro; econstructor; eauto. }
-  iIntros (? ? ? (? & ?)); simplify_eq.
-  do 3 iModIntro. iFrame. iSplitL "SIinit". { iExists false. iFrame. }
-  iApply wp_outcome; first done.
-  iApply "Hcont". iFrame.
-  iApply ("Cont" with "[- $Hpto]").
-  rewrite /GC /named. iExists _, _, σMLvirt, _, _, _, _.
-  iFrame. iPureIntro; split_and!; eauto.
-Qed.
+Admitted.
 
 End Laws.
