theories/interop/wp_prims/registerroot.v
@@ -31,19 +31,11 @@ Proof using.
 
   iApply wp_pre_cases_c_prim; [done..|].
 
-  iAssert (⌜Forall (λ r,
-    ∀ k lv, r !! k = Some lv
-    → ∃ w, mem !! k = Some (Storing w) ∧ repr_lval (θC ρc) lv w)
-  roots_m⌝)%I as "%Hroots".
-  { admit. }
-  destruct (make_repr (θC ρc) roots_m mem) as [privmem Hpriv]; try done.
-  destruct (repr_not_empty (θC ρc) roots_m privmem mem Hpriv) as [rootsChd [rootsCtl Hroots_m]].
-
-  iAssert (⌜¬ l ∈ dom rootsChd⌝)%I as "%Hdom".
-  { admit. }
-    (* iIntros "%H". eapply elem_of_dom in H. destruct H as [k Hk]. *)
-    (* iPoseProof (big_sepM_lookup_acc with "GCrootspto") as "((%ww&Hww&_)&_)". *)
-    (* 1: apply Hk. iPoseProof (resources.mapsto_ne with "Hpto Hww") as "%Hne". congruence. } *)
+  iDestruct "GCrootspto" as "(GCrootsptog&GCrootsptol)".
+  iAssert (⌜¬ l ∈ dom roots_gm⌝)%I as "%Hdom".
+    { iIntros "%H". eapply elem_of_dom in H. destruct H as [k Hk].
+    iPoseProof (big_sepM_lookup_acc with "GCrootsptog") as "((%ww&Hww&_)&_)".
+    1: apply Hk. iPoseProof (resources.mapsto_ne with "Hpto Hww") as "%Hne". congruence. }
 
   iExists (λ '(e', σ'),
     e' = WrSE (ExprO (OVal #0)) ∧
@@ -51,16 +43,16 @@ Proof using.
       χC := χC ρc;
       ζC := ζC ρc;
       θC := θC ρc;
-      rootsC := ({[l]} ∪ (dom rootsChd)) :: (map dom rootsCtl)
+      rootsC := ({[l]} ∪ (dom roots_gm)) :: (map dom roots_fm)
    |} mem).
-  iSplit. { iPureIntro. econstructor; eauto. rewrite <- H2. rewrite Hroots_m. by simpl. }
+  iSplit. { iPureIntro. econstructor; eauto. }
   iIntros (w' ρc' mem' (? & ?)); simplify_eq.
   iMod (ghost_var_update_halves with "SIroots GCroots") as "(SIroots&GCroots)".
-  iMod (ghost_map_insert with "GCrootsm") as "(GCrootsm&Hres)".
+  iMod (ghost_map_insert with "GCrootsg") as "(GCrootsg&Hres)".
   1: eapply not_elem_of_dom; intros Hc; eapply Hdom; done.
   iPoseProof (big_sepM_insert) as "(_&HR)".
   1: eapply not_elem_of_dom; intros Hc; eapply Hdom; done.
-  iPoseProof ("HR" with "[Hpto GCrootspto]") as "GCrootspto"; first iFrame "GCrootspto".
+  iPoseProof ("HR" with "[Hpto GCrootsptog]") as "GCrootsptog"; first iFrame "GCrootsptog".
   1: iExists w; iFrame; done.
   iClear "HR".
   do 3 iModIntro. iFrame. iSplitL "SIinit". { iExists false. iFrame. }
@@ -68,9 +60,11 @@ Proof using.
   iApply "Hcont". iFrame.
   iApply "Cont". iFrame "Hres".
   repeat iExists _. unfold named. iFrame. iPureIntro; split_and!; eauto.
-  - rewrite dom_insert_L. rewrite (_: dom roots_m = rootsC ρc) //.
-  - intros ℓ γ [[-> ->]|[Hne HH]]%lookup_insert_Some; last by eapply Hrootslive.
+  - admit. (* rewrite dom_insert_L. rewrite (_: dom roots_m = rootsC ρc) //. *)
+  - inversion Hrootslive.
+    econstructor; last done.
+    intros ℓ γ [[-> ->]|[Hne HH]]%lookup_insert_Some; last by eapply H1.
     inv_repr_lval. by eapply elem_of_dom_2.
-Qed.
+Admitted.
 
 End Laws.
